Extend sub-typing rules
Adds unrestricted function type, copyable reference type,
and Copy constraint.

.Makefile.coq.d
@@ -4,6 +4,9 @@ theories/lang/subst_map.vos theories/lang/subst_map.vok theories/lang/subst_map.
 theories/lang/hazel.vo theories/lang/hazel.glob theories/lang/hazel.v.beautified theories/lang/hazel.required_vo: theories/lang/hazel.v theories/lang/subst_map.vo
 theories/lang/hazel.vio: theories/lang/hazel.v theories/lang/subst_map.vio
 theories/lang/hazel.vos theories/lang/hazel.vok theories/lang/hazel.required_vos: theories/lang/hazel.v theories/lang/subst_map.vos
-theories/logic/interp.vo theories/logic/interp.glob theories/logic/interp.v.beautified theories/logic/interp.required_vo: theories/logic/interp.v theories/lang/hazel.vo
-theories/logic/interp.vio: theories/logic/interp.v theories/lang/hazel.vio
-theories/logic/interp.vos theories/logic/interp.vok theories/logic/interp.required_vos: theories/logic/interp.v theories/lang/hazel.vos
+theories/logic/interp.vo theories/logic/interp.glob theories/logic/interp.v.beautified theories/logic/interp.required_vo: theories/logic/interp.v theories/lang/hazel.vo theories/logic/iEff.vo
+theories/logic/interp.vio: theories/logic/interp.v theories/lang/hazel.vio theories/logic/iEff.vio
+theories/logic/interp.vos theories/logic/interp.vok theories/logic/interp.required_vos: theories/logic/interp.v theories/lang/hazel.vos theories/logic/iEff.vos
+theories/logic/iEff.vo theories/logic/iEff.glob theories/logic/iEff.v.beautified theories/logic/iEff.required_vo: theories/logic/iEff.v theories/lang/hazel.vo
+theories/logic/iEff.vio: theories/logic/iEff.v theories/lang/hazel.vio
+theories/logic/iEff.vos theories/logic/iEff.vok theories/logic/iEff.required_vos: theories/logic/iEff.v theories/lang/hazel.vos
