theories/logic/interp.v
@@ -9,14 +9,13 @@
 *)
 
 From iris.proofmode Require Import base tactics classes.
-From iris.base_logic.lib Require Import iprop.
+From iris.base_logic.lib Require Import iprop invariants.
 From iris.program_logic Require Import weakestpre.
 From iris Require Import bi.
 From stdpp Require Import base stringmap fin_map_dom fin_maps.
 
 (* Hazel Reasoning *)
-From program_logic Require Import protocols 
-                                  weakest_precondition 
+From program_logic Require Import weakest_precondition 
                                   tactics 
                                   shallow_handler_reasoning 
                                   deep_handler_reasoning 
@@ -24,10 +23,14 @@ From program_logic Require Import protocols
 
 (* Local imports *)
 From affine_tes.lang Require Import hazel.
+From affine_tes.logic Require Import iEff.
+
+
+Context `{!heapGS Σ}.
 
 (** * Semantic Types. *)
 
-Definition sem_ty Σ := val → (iProp Σ).
+Definition sem_ty := val → (iProp Σ).
 
 Declare Scope sem_ty_scope.
 Bind Scope sem_ty_scope with sem_ty.
@@ -35,56 +38,86 @@ Delimit Scope sem_ty_scope with T.
 
 (** * Semantic Row. *)
 
-Definition sem_row Σ := iEff Σ.
+Definition sem_row := iEff Σ.
 
 Declare Scope sem_row_scope.
 Bind Scope ieff_scope with sem_row.
 Delimit Scope sem_row_scope with R.
 
+(* Copyable types *)
+Definition copy_ty (τ : sem_ty) := ∀ v, Persistent (τ v).
+
 (* Base types. *)
-Definition sem_ty_unit {Σ} : sem_ty Σ := (λ v, ⌜ v = #() ⌝)%I.
-Definition sem_ty_bool {Σ} : sem_ty Σ := (λ v, ∃ b : bool, ⌜ v = #b ⌝)%I.
-Definition sem_ty_int {Σ} : sem_ty Σ := (λ v, ∃ n : Z, ⌜ v = #n ⌝)%I.
+Definition sem_ty_unit : sem_ty := (λ v, ⌜ v = #() ⌝)%I.
+Definition sem_ty_bool : sem_ty := (λ v, ∃ b : bool, ⌜ v = #b ⌝)%I.
+Definition sem_ty_int : sem_ty := (λ v, ∃ n : Z, ⌜ v = #n ⌝)%I.
+
+(* Reference Type *)
+Definition tyN := nroot .@ "ty".
+Definition sem_ty_ref (τ : sem_ty): sem_ty := 
+  (λ v, ∃ l : loc, ⌜ v = #l ⌝ ∗ 
+                   inv (tyN .@ l) (∃ w, l ↦ w ∗ ⌜ copy_ty τ ⌝ ∗ □ (τ w)))%I.
 
 (* Product type. *)
-Definition sem_ty_prod {Σ} (A1 A2 : sem_ty Σ) : sem_ty Σ := 
-  (λ v, ∃ v1 v2, ⌜v = (v1, v2)%V⌝ ∗ A1 v1 ∗ A2 v2)%I.
+Definition sem_ty_prod (τ κ : sem_ty) : sem_ty := 
+  (λ v, ∃ v₁ v₂, ⌜v = (v₁, v₂)%V⌝ ∗ τ v₁ ∗ κ v₂)%I.
 
 (* Empty Effect Row. *)
-Definition sem_row_null {Σ} : (sem_row Σ) := iEff_bottom.
+Definition sem_row_bot : sem_row := iEff_bottom.
 
 (* Effect Row. *)
-Definition sem_row_eff {Σ} (A B : sem_ty Σ) : (sem_row Σ) :=
-  (>> (a : val) >> ! a {{ A a }};
-   << (b : val) << ? b {{ B b }} @OS).
+Definition sem_row_eff (τ κ : sem_ty) : sem_row :=
+  (>> (a : val) >> ! a {{ τ a }};
+   << (b : val) << ? b {{ κ b }} @OS).
 
-Lemma upcl_sem_row_eff {Σ} A B v Φ :
-  iEff_car (upcl OS (sem_row_eff (Σ:=Σ) A B)) v Φ ⊣⊢
-    (∃ a, ⌜ v = a ⌝ ∗ A a ∗ (∀ b, B b -∗ Φ b))%I.
+Lemma upcl_sem_row_eff τ κ v Φ :
+  iEff_car (upcl OS (sem_row_eff τ κ)) v Φ ⊣⊢
+    (∃ a, ⌜ v = a ⌝ ∗ τ a ∗ (∀ b, κ b -∗ Φ b))%I.
 Proof. by rewrite /sem_row_eff (upcl_tele' [tele _] [tele _]). Qed.
 
-(* Arrow type. *)
-Definition sem_ty_arr `{!heapGS Σ}
-  (A : sem_ty Σ)
-  (R : sem_row Σ)
-  (B : sem_ty Σ) :=
-  (λ (v : val), ∀ (w : val), A w -∗ EWP (v w) <| R |> {{ B }})%I.
+Lemma sem_row_eff_eq τ κ v Φ :
+  iEff_car (sem_row_eff τ κ) v Φ ⊣⊢
+    (∃ a, ⌜ a = v ⌝ ∗ τ a ∗ (∀ b, κ b -∗ Φ b))%I.
+Proof. by rewrite /sem_row_eff (iEff_tele_eq' [tele _] [tele _]). Qed.
+
+(* Linear Arrow type. *)
+Definition sem_ty_larr
+  (τ : sem_ty)
+  (ρ : sem_row)
+  (κ : sem_ty) : sem_ty :=
+  (λ (v : val), ∀ (w : val), τ w -∗ EWP (v w) <| ρ |> {{ κ }})%I.
+
+(* Unrestricted Arrow type. *)
+Definition sem_ty_uarr
+  (τ : sem_ty)
+  (ρ : sem_row)
+  (κ : sem_ty) : sem_ty :=
+  (λ (v : val), ∀ (w : val), □ (τ w -∗ EWP (v w) <| ρ |> {{ κ }} ))%I.
+
 
 (* Notations. *)
 Notation "()" := sem_ty_unit : sem_ty_scope.
 Notation "'𝔹'" := (sem_ty_bool) : sem_ty_scope.
 Notation "'ℤ'" := (sem_ty_int) : sem_ty_scope.
-Infix "*" := sem_ty_prod : sem_ty_scope.
+Notation "τ '×' κ" := (sem_ty_prod τ%T κ%T)
+  (at level 120, κ at level 200) : sem_ty_scope.
 
-Notation "⟨⟩" := sem_row_null : sem_row_scope.
-Notation "A ⇒ B" := (sem_row_eff A B) 
-  (at level 100, B at level 200) : sem_row_scope.
+Notation "'Ref' τ" := (sem_ty_ref τ%T) 
+  (at level 50) : sem_ty_scope.
 
-Notation "A '-{' R '}-∘' B" := (sem_ty_arr A%T R%R B%T)
-  (at level 100, R, B at level 200) : sem_ty_scope.
-Notation "A ⊸ B" := (sem_ty_arr A%T sem_row_null B%T)
-  (at level 99, B at level 200) : sem_ty_scope.
+Notation "⟨⟩" := sem_row_bot : sem_row_scope.
+Notation "τ ⇒ κ" := (sem_row_eff τ%T κ%T) 
+  (at level 100, κ at level 200) : sem_row_scope.
 
+Notation "τ '-{' ρ '}-∘' κ" := (sem_ty_larr τ%T ρ%R κ%T)
+  (at level 100, ρ, κ at level 200) : sem_ty_scope.
+Notation "τ ⊸ κ" := (sem_ty_larr τ%T sem_row_bot κ%T)
+  (at level 99, κ at level 200) : sem_ty_scope.
+
+Notation "τ '-{' ρ '}->' κ" := (sem_ty_uarr τ%T ρ%R κ%T)
+  (at level 100, ρ, κ at level 200) : sem_ty_scope.
+Notation "τ → κ" := (sem_ty_uarr τ%T sem_row_bot κ%T)
+  (at level 99, κ at level 200) : sem_ty_scope.
 
 (** The Type Context
 
@@ -112,25 +145,25 @@ the same variable occurs twice in Γ we get that:
 
 *) 
 
-Notation ctx Σ := (list (string * (sem_ty Σ))).
+Notation ctx := (list (string * sem_ty)).
 
 (** The domain of the context. *)
-Definition ctx_dom Σ : ctx Σ -> list string := map fst.
+Notation ctx_dom := (map fst).
 
-Fixpoint ctx_sem_typed Σ (Γ : ctx Σ)
-                         (vs : gmap string val) : iProp Σ :=
+Fixpoint ctx_sem_typed (Γ : ctx)
+                       (vs : gmap string val) : iProp Σ :=
   match Γ with
-    | [] => True
+    | [] => emp
     | (x,A) :: Γ' => (∃ v, ⌜ vs !! x = Some v ⌝ ∗ A v) ∗ 
-                     ctx_sem_typed Σ Γ' vs
+                     ctx_sem_typed Γ' vs
   end.
 
-Lemma ctx_sem_typed_empty Σ vs : ⊢ ctx_sem_typed Σ [] vs.
+Lemma ctx_sem_typed_empty vs : ⊢ ctx_sem_typed [] vs.
 Proof. done. Qed.
 
-Lemma ctx_sem_typed_insert Σ Γ vs (x : string) v :
-  x ∉ (ctx_dom Σ Γ) →
-  ctx_sem_typed Σ Γ vs ⊢ ctx_sem_typed Σ Γ (binder_insert x v vs).
+Lemma ctx_sem_typed_insert Γ vs (x : string) v :
+  x ∉ (ctx_dom Γ) →
+  ctx_sem_typed Γ vs ⊢ ctx_sem_typed Γ (binder_insert x v vs).
 Proof.
   iIntros (Helem) "Henv".
   iInduction Γ as [|[y A] Γ'] "IH"; first done. simpl in *.
@@ -140,31 +173,231 @@ Proof.
     { destruct Helem. by apply elem_of_list_here. }
     by rewrite lookup_insert_ne.
   - iApply "IH"; last done. iPureIntro. 
-    destruct (not_elem_of_cons (ctx_dom Σ Γ') x y) as [[ ] _]; done.
+    destruct (not_elem_of_cons (ctx_dom Γ') x y) as [[ ] _]; done.
 Qed.
 
-Lemma ctx_sem_typed_app Σ Γ₁ Γ₂ vs :
-  ctx_sem_typed Σ (Γ₁ ++ Γ₂) vs ⊢ 
-  ctx_sem_typed Σ Γ₁ vs ∗ ctx_sem_typed Σ Γ₂ vs.
+Lemma ctx_sem_typed_app Γ₁ Γ₂ vs :
+  ctx_sem_typed (Γ₁ ++ Γ₂) vs ⊢ 
+  ctx_sem_typed Γ₁ vs ∗ ctx_sem_typed Γ₂ vs.
 Proof. 
   iIntros "HΓ₁₂". iInduction Γ₁ as [|[y A] Γ₁'] "IH"; first (by iFrame).
   simpl in *. 
   iDestruct "HΓ₁₂" as "($ & HΓ₁'₂)". by iApply "IH".
 Qed.
 
+Definition copy_ctx Γ :=
+  ∀ vs, Persistent (ctx_sem_typed Γ vs).
 
-Section semantic_typing_rules.
 
-Context `{!heapGS Σ}.
+(* Sub-typing and relations *)
+
+Definition ty_le (A B : sem_ty) := ∀ v, A v ⊢ B v.
+Definition row_le (ρ ρ' : sem_row) := ⊢ iEff_le ρ ρ'.
+Definition ctx_le Γ₁ Γ₂ :=
+  ∀ vs, ctx_sem_typed Γ₁ vs ⊢ ctx_sem_typed Γ₂ vs.
+
+Notation "Γ₁ '≤C' Γ₂" := (ctx_le Γ₁ Γ₂) (at level 98).
+Notation "τ '≤T' κ" := (ty_le τ%T κ%T) (at level 98).
+
+Notation "ρ '≤R' ρ'" := (row_le ρ%R ρ'%R) (at level 98).
+
+Lemma row_le_refl (ρ : sem_row) : ρ ≤R ρ.
+Proof. iApply iEff_le_refl. Qed.
+
+Lemma row_le_trans (ρ₁ ρ₂ ρ₃: sem_row) : 
+    ρ₁ ≤R ρ₂ →
+    ρ₂ ≤R ρ₃ →
+    ρ₁ ≤R ρ₃. 
+Proof. 
+  intros Hρ₁₂ Hρ₂₃. 
+  iApply iEff_le_trans; [iApply Hρ₁₂|iApply Hρ₂₃]. 
+Qed.
+
+Lemma row_le_bot (ρ : sem_row) :
+  ⟨⟩ ≤R ρ.
+Proof. iApply iEff_le_bottom. Qed.
+
+Lemma row_le_eff (ι₁ ι₂ κ₁ κ₂ : sem_ty) :
+  ι₁ ≤T ι₂ →
+  κ₂ ≤T κ₁ →
+  ((ι₁ ⇒ κ₁) ≤R (ι₂ ⇒ κ₂)).
+Proof.
+  iIntros (Hι₁₂ Hκ₂₁ v) "%Φ !#".
+  rewrite !sem_row_eff_eq.
+  iIntros "(%a & -> & Hι₁ & HκΦ₁)".
+  iExists v. iSplit; first done. iSplitL "Hι₁".
+  { by iApply Hι₁₂. }
+  iIntros (b) "Hκ₂". iApply "HκΦ₁".
+  by iApply Hκ₂₁.
+Qed.
+
+Lemma ty_le_refl (τ : sem_ty) : τ ≤T τ.
+Proof. done. Qed.
+
+Lemma ty_le_trans (τ₁ τ₂ τ₃ : sem_ty) :
+  τ₁ ≤T τ₂ →
+  τ₂ ≤T τ₃ →
+  τ₁ ≤T τ₃.
+Proof. 
+  iIntros (Hτ₁₂ Hτ₂₃ v) "Hτ₁". 
+  iApply Hτ₂₃. by iApply Hτ₁₂.
+Qed.
+
+Lemma ty_le_arr (τ κ : sem_ty) (ρ : sem_row) :
+  (τ -{ ρ }-> κ) ≤T (τ -{ ρ }-∘ κ).
+Proof.
+  iIntros (v) "#Hτκ %w Hw".
+  iApply (ewp_mono with "[Hw]").
+  { by iApply "Hτκ". }
+  iIntros (u) "Hu". by iModIntro.
+Qed.
+
+Lemma ty_le_larr (τ₁ κ₁ τ₂ κ₂ : sem_ty) (ρ ρ' : sem_row) :
+  ρ ≤R ρ' →
+  τ₂ ≤T τ₁ →
+  κ₁ ≤T κ₂ →
+  (τ₁ -{ ρ }-∘ κ₁) ≤T (τ₂ -{ ρ' }-∘ κ₂).
+Proof.
+  iIntros (Hρ Hτ₂₁ Hκ₁₂ v) "Hτκ₁ %w Hw".
+  iApply ewp_os_prot_mono.
+  { iApply Hρ. }
+  iApply (ewp_mono with "[Hw Hτκ₁]").
+  { iApply "Hτκ₁". by iApply Hτ₂₁. }
+  iIntros (u) "Hu". iModIntro. by iApply Hκ₁₂.
+Qed.
+
+Lemma ty_le_uarr (τ₁ κ₁ τ₂ κ₂ : sem_ty) (ρ ρ' : sem_row) :
+  ρ ≤R ρ' →
+  τ₂ ≤T τ₁ →
+  κ₁ ≤T κ₂ →
+  (τ₁ -{ ρ }-> κ₁) ≤T (τ₂ -{ ρ' }-> κ₂).
+Proof.
+  iIntros (Hρ Hτ₂₁ Hκ₁₂ v) "#Hτκ₁ %w !# Hw".
+  iApply ewp_os_prot_mono.
+  { iApply Hρ. }
+  iApply (ewp_mono with "[Hw]").
+  { iApply "Hτκ₁". by iApply Hτ₂₁. }
+  iIntros (u) "Hu". iModIntro. by iApply Hκ₁₂.
+Qed.
+
+Lemma ty_le_prod (τ₁ τ₂ κ₁ κ₂ : sem_ty) :
+  τ₁ ≤T τ₂ →
+  κ₁ ≤T κ₂ →
+  (τ₁ × κ₁) ≤T (τ₂ × κ₂).
+Proof.
+  iIntros (Hτ₁₂ Hκ₁₂ v) "(%w₁ & %w₂ & -> &Hw₁ & Hw₂)".
+  iExists w₁, w₂. iSplit; first done. iSplitL "Hw₁".
+  { by iApply Hτ₁₂. }
+  by iApply Hκ₁₂.
+Qed.
+
+Lemma ctx_le_refl Γ : Γ ≤C Γ.
+Proof. done. Qed.
+
+Lemma ctx_le_trans Γ₁ Γ₂ Γ₃ : 
+  Γ₁ ≤C Γ₂ →
+  Γ₂ ≤C Γ₃ →
+  Γ₁ ≤C Γ₃.
+Proof.
+  iIntros (HΓ₁₂ HΓ₂₃ vs) "HΓ₁ //=".  
+  iApply HΓ₂₃. by iApply HΓ₁₂.
+Qed.
+
+Lemma ctx_le_cons Γ₁ Γ₂ τ₁ τ₂ x :
+  Γ₁ ≤C Γ₂ →
+  τ₁ ≤T τ₂ →
+  (x, τ₁) :: Γ₁ ≤C (x, τ₂) :: Γ₂.
+Proof.
+  iIntros (HΓ₁₂ Hτ₁₂ vs) "//= ((%v & Hlookup & Hv) & HΓ₁)".
+  iSplitR "HΓ₁"; last (by iApply HΓ₁₂).
+  iExists v. iFrame. by iApply Hτ₁₂.
+Qed.
+
+Lemma ctx_le_copy_contraction Γ x τ :
+  copy_ty τ →
+  (x, τ) :: Γ ≤C (x, τ) :: (x, τ) :: Γ.
+Proof.
+  iIntros (Hcpyτ vs) "//= [(%w & -> & Hτ) $]". 
+  rewrite Hcpyτ. iDestruct "Hτ" as "#Hτ".
+  iSplitL; iExists w; by iSplit.
+Qed.
+
+Lemma ctx_le_swap Γ x y τ κ :
+  (x, τ) :: (y, κ) :: Γ ≤C (y, κ) :: (x, τ) :: Γ.
+Proof. iIntros (vs) "($ & $ & $) //=". Qed.
+
+(* Copyable types *)
+
+Lemma copy_ty_unit : copy_ty ().
+Proof. 
+  iIntros (v). apply bi.pure_persistent.
+Qed.
+
+Lemma copy_ty_bool : copy_ty 𝔹.
+Proof. 
+  iIntros (v).
+  apply bi.exist_persistent. iIntros (x).
+  apply bi.pure_persistent.
+Qed.
+
+Lemma copy_ty_nat : copy_ty ℤ.
+Proof. 
+  iIntros (v). 
+  apply bi.exist_persistent. iIntros (x).
+  apply bi.pure_persistent.
+Qed.
+
+Lemma copy_ty_ref τ : copy_ty (Ref τ).
+Proof.
+  iIntros (v). unfold sem_ty_ref.
+  apply bi.exist_persistent. iIntros (x).
+  apply bi.sep_persistent.
+  { apply bi.pure_persistent. }
+  apply inv_persistent.
+Qed.
+
+Lemma copy_ty_uarr τ ρ κ : copy_ty (τ -{ ρ }-> κ).
+Proof.
+  iIntros (v). unfold sem_ty_uarr.
+  apply bi.forall_persistent. iIntros (x).
+  apply bi.intuitionistically_persistent.
+Qed.
+
+Lemma copy_ty_prod τ κ : copy_ty τ → copy_ty κ → copy_ty (τ × κ).
+Proof.
+  iIntros (Hcpyτ Hcpyκ v). unfold sem_ty_prod.
+  do 2 (apply bi.exist_persistent; iIntros (?)).
+  apply bi.sep_persistent; [apply bi.pure_persistent|].
+  apply bi.sep_persistent.
+  { apply Hcpyτ. }
+  apply Hcpyκ. 
+Qed.
+
+Lemma copy_ctx_nil : copy_ctx [].
+Proof. iIntros (vs). apply bi.emp_persistent. Qed.
+
+Lemma copy_ctx_cons Γ x τ : 
+  copy_ctx Γ →
+  copy_ty τ →
+  copy_ctx ((x, τ) :: Γ).
+Proof. 
+  iIntros (HcpyΓ Hcpyτ vs). simpl.
+  apply bi.sep_persistent; last done.
+  apply bi.exist_persistent. intros v.
+  apply bi.sep_persistent; last done.
+  apply bi.pure_persistent.
+Qed.
+
+(** Semantic typing rules *)
 
 (* Semantic typing judgment. *)
 Definition sem_typed 
-  (Γ  : ctx Σ)
+  (Γ  : ctx)
   (e  : expr)
-  (ρ  : sem_row Σ)
-  (α  : sem_ty Σ) : Prop :=
+  (ρ  : sem_row)
+  (α  : sem_ty) : Prop :=
     ∀ (vs : gmap string val),
-        ctx_sem_typed Σ Γ vs ⊢ EWP (subst_map vs e) <| ρ |> {{ α }}.
+        ctx_sem_typed Γ vs ⊢ EWP (subst_map vs e) <| ρ |> {{ α }}.
 
 Notation "Γ ⊨ e : ρ : α" := (sem_typed Γ e%E ρ%R α%T)
   (at level 74, e, ρ, α at next level) : bi_scope.
@@ -179,47 +412,70 @@ Open Scope ieff_scope.
 
 (* Base rules *)
 
-Lemma sem_typed_unit Γ ρ : 
-  Γ ⊨ #() : ρ : ().
+Lemma sem_typed_unit Γ : 
+  Γ ⊨ #() : ⟨⟩ : ().
 Proof.
   iIntros (vs) "HΓ //=". by iApply ewp_value.
 Qed.
 
-Lemma sem_typed_bool Γ ρ (b : bool) : 
-  Γ ⊨ #b : ρ : 𝔹.
+Lemma sem_typed_bool Γ (b : bool) : 
+  Γ ⊨ #b : ⟨⟩ : 𝔹.
 Proof.
   iIntros (vs) "HΓ //=". iApply ewp_value. by iExists b.
 Qed.
 
-Lemma sem_typed_int Γ ρ (i : Z) : 
-  Γ ⊨ #i : ρ : ℤ.
+Lemma sem_typed_int Γ (i : Z) : 
+  Γ ⊨ #i : ⟨⟩ : ℤ.
 Proof.
   iIntros (vs) "HΓ //=". iApply ewp_value. by iExists i.
 Qed.
 
 (* Subsumption rule *)
 
-Lemma sem_typed_sub Γ e τ ρ: 
-  Γ ⊨ e: ⟨⟩ : τ →
-  Γ ⊨ e: ρ : τ.
+Lemma sem_typed_sub Γ Γ' e ρ ρ' τ τ':
+  Γ' ≤C Γ →
+  ρ  ≤R ρ' → 
+  τ  ≤T τ' →
+  Γ ⊨ e: ρ : τ →
+  Γ' ⊨ e: ρ' : τ'.
 Proof.
-  iIntros (He vs) "HΓ //=".
+  iIntros (HΓle Hρle Hτle He vs) "HΓ' //=".
+  rewrite HΓle.
   iApply ewp_os_prot_mono.
-  { iApply iEff_le_bottom. }
-  by iApply He.
+  { iApply Hρle. }
+  iApply (ewp_mono with "[HΓ']").
+  { by iApply He. }
+  iIntros (v) "Hτ". iModIntro.
+  by iApply Hτle.
 Qed.
 
 (* λ-calculus rules *)
 
-Lemma sem_typed_fun Γ x e τ ρ κ: 
-  x ∉ (ctx_dom Σ Γ) →
+Lemma sem_typed_lfun Γ x e τ ρ κ: 
+  x ∉ (ctx_dom Γ) →
   (x,τ) :: Γ ⊨ e : ρ : κ →
   Γ ⊨ (λ: x, e) : ⟨⟩ : (τ -{ ρ }-∘ κ).
 Proof.
   iIntros (Helem He vs) "HΓ //=".
-  ewp_pure_steps. iIntros (w) "Hτw". ewp_pure_steps. 
+  ewp_pure_steps. iIntros (w) "Hw". ewp_pure_steps. 
   rewrite <- subst_map_insert.
-  iApply He. simpl in *. iSplitL "Hτw".
+  iApply He. simpl in *. iSplitL "Hw".
+  - iExists w. iFrame. iPureIntro.
+    by rewrite lookup_insert.
+  - by iApply ctx_sem_typed_insert.
+Qed.
+
+Lemma sem_typed_ufun Γ x e τ ρ κ: 
+  x ∉ (ctx_dom Γ) →
+  copy_ctx Γ →
+  (x,τ) :: Γ ⊨ e : ρ : κ →
+  Γ ⊨ (λ: x, e) : ⟨⟩ : (τ -{ ρ }-> κ).
+Proof.
+  iIntros (Helem HcpyΓ He vs) "HΓ //=".
+  ewp_pure_steps. rewrite HcpyΓ. iDestruct "HΓ" as "#HΓ".
+  iIntros (w) "!# Hw". ewp_pure_steps. 
+  rewrite <- subst_map_insert.
+  iApply He. simpl in *. iSplitL "Hw".
   - iExists w. iFrame. iPureIntro.
     by rewrite lookup_insert.
   - by iApply ctx_sem_typed_insert.
@@ -246,7 +502,7 @@ Qed.
 Lemma sem_typed_pair Γ₁ Γ₂ e₁ e₂ τ ρ κ: 
   Γ₁ ⊨ e₁ : ρ : τ →
   Γ₂ ⊨ e₂ : ρ : κ →
-  Γ₁ ++ Γ₂ ⊨ (e₁,e₂) : ρ : τ * κ.
+  Γ₁ ++ Γ₂ ⊨ (e₁,e₂) : ρ : (τ × κ).
 Proof.
   iIntros (He₁ He₂ vs) "HΓ₁₂ //=".
   rewrite ctx_sem_typed_app.
@@ -263,10 +519,10 @@ Proof.
 Qed.
 
 Lemma sem_typed_pair_elim Γ₁ Γ₂ x₁ x₂ e₁ e₂ τ ρ κ ι: 
-  x₁ ∉ (ctx_dom Σ Γ₂) ->
-  x₂ ∉ (ctx_dom Σ Γ₂) ->
+  x₁ ∉ (ctx_dom Γ₂) ->
+  x₂ ∉ (ctx_dom Γ₂) ->
   x₁ ≠ x₂ ->
-  Γ₁ ⊨ e₁ : ρ : (τ * κ) →
+  Γ₁ ⊨ e₁ : ρ : (τ × κ) →
   (x₁, τ) :: (x₂, κ) :: Γ₂ ⊨ e₂ : ρ : ι →
   Γ₁ ++ Γ₂ ⊨ (let: (x₁, x₂) := e₁ in e₂) : ρ : ι.
 Proof.
@@ -314,6 +570,84 @@ Proof.
   destruct b; ewp_pure_steps.
   - by iApply He₂.
   - by iApply He₃.
+Qed.
+
+(* reference rules *)
+
+(* The references that we implement here are always copyable, 
+   so we have ∀ τ, copy_ty (Ref τ).
+   This allows us to treat references in a non sub-structural way.
+   Since we do not have `free` in our language
+   we do not have use-after-free and double-free problems
+   and so making them persistent will be too restrictive.
+   This is why the `load` does not return the reference back
+   and we can always `load` from the same reference more than once.
+
+   The down side of this is that we cannot store
+   non-persistent functions like continuations.
+*)
+   
+Lemma sem_typed_alloc Γ e ρ τ: 
+  copy_ty τ →
+  Γ ⊨ e : ρ : τ →
+  Γ ⊨ ref e : ρ : Ref τ.
+Proof.
+  iIntros (Hcpyτ He vs) "HΓ //=".
+  iApply (ewp_bind [AllocCtx]); first done. simpl.
+  iApply (ewp_mono with "[HΓ]").
+  { by iApply He. }
+  iIntros (v) "Hτ". iModIntro.
+  iApply ewp_alloc. iIntros "!> %l Hl".
+  iMod (inv_alloc (tyN.@l) _
+       (∃ w, l ↦ w ∗ ⌜copy_ty τ⌝ ∗ □ τ w)%I with "[Hl Hτ]") as "#Hinv".
+  { iExists v. iFrame. iSplit; first done.
+    by iApply bi.intuitionistic. }
+  iModIntro. iExists l. by auto.
+Qed.
+
+Lemma sem_typed_load Γ e ρ τ: 
+  Γ ⊨ e : ρ : Ref τ →
+  Γ ⊨ !e : ρ : τ.
+Proof.
+  iIntros (He vs) "HΓ //". simpl.
+  iApply (ewp_bind [LoadCtx]); first done. simpl.
+  iApply (ewp_mono with "[HΓ]").
+  { by iApply He. }
+  iIntros (v) "(%l & -> & #Hinv)". iModIntro.
+  iApply (ewp_atomic _ (⊤ ∖ ↑tyN.@l)).
+  iMod (inv_acc _ (tyN.@l) with "Hinv") as "[(%w & >Hl & >%Hcpy & HA) Hclose]"; 
+    first done.
+  iModIntro. iApply (ewp_load with "Hl").
+  iNext. iDestruct "HA" as "#HA". 
+  iIntros "Hl !>". simpl.
+  iMod ("Hclose" with "[Hl]"); last done.
+  iExists w. iFrame. by iSplit.
+Qed.
+
+Lemma sem_typed_store Γ₁ Γ₂ e₁ e₂ ρ τ: 
+  Γ₁ ⊨ e₁ : ρ : Ref τ →
+  Γ₂ ⊨ e₂ : ρ : τ →
+  Γ₁ ++ Γ₂ ⊨ (e₁ <- e₂) : ρ : ().
+Proof.
+  iIntros (He₁ He₂ vs) "HΓ₁₂ //=".
+  rewrite !ctx_sem_typed_app.
+  iDestruct "HΓ₁₂" as "(HΓ₁ & HΓ₂)". 
+  iApply (ewp_bind [StoreRCtx _]); first done. simpl.
+  iApply (ewp_mono with "[HΓ₂]").
+  { by iApply He₂. }
+  iIntros (v) "Hτ". iModIntro.
+  iApply (ewp_bind [StoreLCtx _]); first done. simpl.
+  iApply (ewp_mono with "[HΓ₁]").
+  { by iApply He₁. }
+  iIntros (w) "(%l & -> & #Hinv)". iModIntro.
+  iApply (ewp_atomic _ (⊤ ∖ ↑tyN.@l)).
+  iMod (inv_acc _ (tyN.@l) with "Hinv") as "[(%w & >Hl & >%Hcpy & HA) Hclose]"; 
+    first done.
+  iModIntro. iApply (ewp_store with "Hl").
+  iIntros "!> Hl !>". 
+  iMod ("Hclose" with "[Hl Hτ]"); last done.
+  iExists v. iFrame. iSplit; first done.
+  by iApply bi.intuitionistic.
 Qed.
 
 (* Effect handling rules *)
@@ -415,20 +749,21 @@ Qed.
       return (λ v, v) 
    end / l ↦ #false
  *)
-Lemma sem_typed_deep_try Γ₁ Γ₂ e (h : val) r ρ' ι κ τ τ': 
+Lemma sem_typed_deep_try Γ₁ Γ₂ Γ₃ e (h : val) r ρ' ι κ τ τ': 
+  copy_ctx Γ₂ →
   let ρ := (ι ⇒ κ)%R in
   Γ₁ ⊨ e : ρ : τ →
-  ⊨ (of_val h) : ⟨⟩ : (ι ⊸ (κ -{ ρ' }-∘ τ') -{ ρ' }-∘ τ') →
-  Γ₂ ⊨ r : ⟨⟩ : (τ -{ ρ' }-∘ τ') →
-  Γ₁ ++ Γ₂ ⊨ (deep-try: e with effect h | return r end) : ρ' : τ'.
+  Γ₂ ⊨ (of_val h) : ⟨⟩ : (ι ⊸ (κ -{ ρ' }-∘ τ') -{ ρ' }-∘ τ') →
+  Γ₃ ⊨ r : ⟨⟩ : (τ -{ ρ' }-∘ τ') →
+  Γ₁ ++ Γ₂ ++ Γ₃ ⊨ (deep-try: e with effect h | return r end) : ρ' : τ'.
 Proof.
-  iIntros (ρ He Hh Hr vs) "HΓ₁₂ //=".
-  rewrite ctx_sem_typed_app.
-  iDestruct "HΓ₁₂" as "[HΓ₁ HΓ₂]". ewp_pure_steps.
+  iIntros (Hcpy ρ He Hh Hr vs) "HΓ₁₂₃ //=".
+  rewrite !ctx_sem_typed_app. rewrite Hcpy.
+  iDestruct "HΓ₁₂₃" as "(HΓ₁ & #HΓ₂ & HΓ₃)". ewp_pure_steps.
   set rctx := AppRCtx (deep_try_with (λ: <>, subst_map vs e)%E (subst_map vs h))%E.
   iApply (ewp_bind [rctx]); first done.
   iApply ewp_os_prot_mono; [by iApply iEff_le_bottom|].
-  iApply (ewp_mono with "[HΓ₂]").
+  iApply (ewp_mono with "[HΓ₃]").
   { by iApply Hr. }
   iIntros (r') "Hr'". iModIntro. simpl.
   ewp_pure_steps.
@@ -445,7 +780,7 @@ Proof.
     iApply (ewp_bind [AppLCtx k; AppLCtx a]); first done. 
     iApply ewp_os_prot_mono; [by iApply iEff_le_bottom|]. 
     simpl. iApply ewp_mono.
-    { iApply Hh. iApply (ctx_sem_typed_empty _ empty). }
+    { by iApply Hh. }
     iIntros (h') "Hh'". iModIntro. simpl.
     iApply (ewp_bind [AppLCtx k]); first done. simpl.
     iApply ewp_os_prot_mono; [by iApply iEff_le_bottom|]. 
@@ -457,5 +792,3 @@ Proof.
     rewrite !deep_handler_unfold. 
     iApply ("IH" with "Hr'").
   Qed.
-
-End semantic_typing_rules.
