theories/lang/hazel.v
@@ -5,6 +5,9 @@
    the let-pair construct and its eliminator.
 *)
 
+From iris.program_logic Require Export language.
+From iris.heap_lang     Require Export locations.
+
 (* Hazel language *)
 From language Require Export eff_lang.
 
@@ -20,3 +23,34 @@ Notation ELetPair x1 x2 e1 e2 :=
 Notation "'let:' '(' x1 ',' x2 ')' := e1 'in' e2" := (ELetPair x1%binder x2%binder e1%E e2%E)
   (at level 200, x1, x2 at level 1, e1, e2 at level 200,
    format "'[' 'let:'  '(' x1 ',' x2 ')'  :=  '[' e1 ']'  'in'  '/' e2 ']'") : expr_scope.
+
+Global Instance load_atomic (l : loc) :
+  Atomic StronglyAtomic (Load $ Val $ LitV $ LitLoc l).
+Proof.
+  intros ?. simpl. intros ?????. unfold prim_step' in H.
+  destruct κ; [|done].
+  destruct efs; [|done]. inversion H. simplify_eq.
+  destruct k as [|Ki K]; try destruct Ki; try naive_solver.
+  - simpl in H0. simpl. simplify_eq. inversion H2. by exists v.
+  - simpl in H0. simpl. simplify_eq.
+    destruct K as [|Ki K]; try destruct Ki; try naive_solver.
+    simpl in H0. simplify_eq. by inversion H2.
+Qed.
+
+Global Instance store_atomic (l : loc) (w : val) :
+  Atomic StronglyAtomic (Store (Val $ LitV $ LitLoc l) (Val w)).
+Proof.
+ intros ?. simpl. intros ?????. unfold prim_step' in H.
+ destruct κ; [|done].
+ destruct efs; [|done]. inversion H. simplify_eq.
+ destruct k as [|Ki K]; try destruct Ki; try naive_solver.
+ - simpl in H0. simpl. simplify_eq. inversion H2.
+   by exists (LitV $ LitUnit).
+ - simpl in H0. simpl. simplify_eq.
+   destruct K as [|Ki K]; try destruct Ki; try naive_solver.
+   simpl in H0. simplify_eq. by inversion H2.
+ - simpl in H0. simpl. simplify_eq.
+   destruct K as [|Ki K]; try destruct Ki; try naive_solver.
+   simpl in H1. simplify_eq. by inversion H2.
+Qed.
+
