theories/logic/iEff.v
@@ -1,0 +1,24 @@
+
+From iris.proofmode  Require Import tactics.
+From iris.base_logic Require Export lib.iprop.
+
+From program_logic Require Export protocols.
+From affine_tes.lang Require Import hazel.
+
+
+Lemma iEff_tele_eq' {Σ} (TT1 TT2 : tele) v m
+  (v' : TT1 -t>         val) (P : TT1 -t>         iProp Σ)
+  (w' : TT1 -t> TT2 -t> val) (Q : TT1 -t> TT2 -t> iProp Σ) Φ :
+  iEff_car
+    (>>.. x >> !           (tele_app v' x)
+               {{          (tele_app P  x)   }};
+     <<.. y << ? (tele_app (tele_app w' x) y)
+               {{ tele_app (tele_app Q  x) y }} @m) v Φ ≡
+  (∃.. x, ⌜ tele_app v' x = v ⌝ ∗ tele_app P x ∗
+    □? m (∀.. y, tele_app (tele_app Q  x) y -∗
+          Φ (tele_app (tele_app w' x) y)))%I.
+Proof. by rewrite (iEff_tele_eq (tele_app v') (tele_app P)
+                  (λ x y, tele_app (tele_app w' x) y)
+                  (λ x y, tele_app (tele_app Q  x) y)).
+Qed.
+
